rustfrontend/BorrowCheckInv.v
@@ -11,14 +11,11 @@ Require Import Rusttypes Rustlight.
 Require Import RustOp RustIR Rusttyping.
 Require Import Errors.
 Require Import Listmisc.
-Require Import BorrowCheck.
-Require Import MoveCheckingFootprint1.
-(* Unsupported for now *)
-(* Require Import StkBorPermission RustIRbor. *)
 Require Import RustIRspec.
-Require Import BorrowCheckDomain RegionLiveness.
 
 Import ListNotations.
+
+Local Open Scope error_monad_scope.
 
 Section ADT_ENV.
 
@@ -26,103 +23,95 @@ Context {ame: adt_mem_env}.
 
 Notation footprint := (@footprint ame).
 Notation fp_map := (@fp_map ame).
-Notation ae := (fun id => (ame id).(mem_pure_adt)).
-Notation sval := (@sval ae).
-Notation sv_map := (@sv_map ae).
+Notation get_owner_path_map := (@get_owner_path_map ame).
+
+(* Section COMP_ENV. *)
+
+(* Variable ce: composite_env. *)
+
+(* Fixpoint mutable_projections (ty: type) (phl: list projection) : bool := *)
+(*   match phl with *)
+(*   | nil => true *)
+(*   | ph :: phl1 => *)
+(*       match ph with *)
+(*       | proj_deref =>  *)
+(*           if is_immutable_ref ty then  *)
+(*             false *)
+(*           else  *)
+(*             match type_deref ty with *)
+(*             | OK ty1 => mutable_projections ty1 phl1 *)
+(*             | _ => false *)
+(*             end *)
+(*       | proj_field fid =>  *)
+(*           match type_field ce ty fid with *)
+(*           | OK ty1 => mutable_projections ty1 phl1 *)
+(*           | _ => false *)
+(*           end *)
+(*       | proj_downcast fid =>  *)
+(*           match type_downcast ce ty fid with *)
+(*           | OK ty1 => mutable_projections ty1 phl1 *)
+(*           | _ => false *)
+(*           end *)
+(*       end *)
+(*   end. *)
 
 
-Section COMP_ENV.
+(* Definition mutable_path (fpm: fp_map) (ph: path) : bool := *)
+(*   let (id, phl) := ph in *)
+(*   match fpm ! id with *)
+(*   | Some (_, _, _, ty, _) => *)
+(*       mutable_projections ty phl *)
+(*   | None => *)
+(*       false *)
+(*   end. *)
 
-Variable ce: composite_env.
+(* End COMP_ENV. *)
 
-Fixpoint mutable_projections (ty: type) (phl: list projection) : bool :=
+Fixpoint mutable_path_footprint (fpg: fp_graph) (phl: list projection) (fp: footprint) : res bool :=
   match phl with
-  | nil => true
-  | ph :: phl1 =>
-      match ph with
-      | proj_deref => 
-          if is_immutable_ref ty then 
-            false
-          else 
-            match type_deref ty with
-            | OK ty1 => mutable_projections ty1 phl1
-            | _ => false
-            end
-      | proj_field fid => 
-          match type_field ce ty fid with
-          | OK ty1 => mutable_projections ty1 phl1
-          | _ => false
+  | nil => OK true
+  | pj :: l =>
+      match pj, fp with
+      | proj_deref , fp_box _ fp1 =>          
+          mutable_path_footprint fpg l fp1
+      | proj_field fid, fp_struct _ fpl =>
+          match find_field fid fpl with
+          | Some (_, ffp) =>
+              mutable_path_footprint fpg l ffp
+          | None => Error nil
           end
-      | proj_downcast fid => 
-          match type_downcast ce ty fid with
-          | OK ty1 => mutable_projections ty1 phl1
-          | _ => false
+      | proj_field fid, fp_object _ _ fpl =>
+          match find_field fid fpl with
+          | Some (_, ffp) =>
+              mutable_path_footprint fpg l ffp
+          | None => Error nil
           end
+      | proj_downcast fid1, fp_enum _ _ fid2 _ fp1 =>
+          if ident_eq fid1 fid2 then
+            mutable_path_footprint fpg l fp1
+          else
+            Error nil
+      | proj_deref, fp_ref mut _ _ (Some ph2) rebor =>
+          match mut with
+          | Mutable =>
+              do fp2 <- get_owner_footprint_map ph2 fpg;
+              mutable_path_footprint fpg l fp2
+          | Immutable =>
+              OK false
+          end
+      | _, _  => Error nil
       end
   end.
 
 
-Definition mutable_path (svm: sv_map) (ph: path) : bool :=
+Definition mutable_path (ph: path) (fpg: fp_graph) : res bool :=
   let (id, phl) := ph in
-  match svm ! id with
-  | Some (_, ty, sv) =>
-      mutable_projections ty phl
-  | None =>
-      false
+  match fpg!id with
+  | Some fp =>
+      mutable_path_footprint fpg phl fp
+  | _ => Error nil
   end.
 
-End COMP_ENV.
-
-Definition is_live_path (live: RegionSet.t) (te: typenv) (ph: path) : bool :=
-  let (id, phl) := ph in
-  match te ! id with
-  | Some ty =>
-      forallb (fun r => RegionSet.mem r live) (origins_of_type ty)
-  | None =>
-      false
-  end.
-
-(* We also need to know that generic region this path locates
-at....  *)
-Definition extern_loc_region (svm: sv_map) (ph: path) : option origin :=
-  let (id, pj) := ph in
-  match svm ! id with
-  | Some (r, _, _) =>
-      r
-  | _ => None
-  end.
-
-(* [ln] is a prefix of [ph] *)
-Definition loan_approx (svm: sv_map) (ln: loan) (ph: path) : Prop :=
-  match ln, extern_loc_region svm ph with
-  | Lintern _ p, None =>
-      (* TODO: maybe we should use path uniformly *)
-      let (id1, pj1) := path_of_place p in
-      let (id2, pj2) := ph in
-      id1 = id2 /\ projections_contain pj1 pj2 = true
-  | Lextern org1, Some org2 =>
-      org1 = org2 
-  | _, _ => False
-  end.
-
-(* ph is the location the reference points to *)
-Definition alias_graph_approx_loans ce (live: RegionSet.t) (ls: LoanSet.t) (svm: sv_map) (vs: views) (ph: path) : Prop :=
-  forall vph vs1,
-    In vph vs ->
-    is_live_path live (svm_to_tenv svm) vph = true ->
-    mutable_path ce svm vph = true ->
-    get_owner_path_sv_map vph svm = OK (ph, vs1) ->
-    exists ln, 
-      LoanSet.In ln ls ->
-      loan_approx svm ln vph.
-
-
-Definition sound_loan_analysis ce (live: RegionSet.t) (le: LOrgEnv.t) (svm: sv_map) : Prop :=
-  forall rph ph vs mut ty ls r,
-    get_owner_sval_map rph svm = OK (sv_ref mut ph vs) ->
-    wt_path ce (svm_to_tenv svm) rph = OK (Treference r mut ty) ->
-    LOrgEnv.get r le = Live ls ->
-    alias_graph_approx_loans ce live ls svm vs ph.
 
 (* Maybe useful comment *)
 (* For safety: all owner paths that have the ability to change the
@@ -142,173 +131,81 @@ precisely(?) capature all reachable paths (that are live and mutable)
 to this reference path excluding the paths created by reborrowed from
 this reference path. *)
 
-Definition alias_graph_views_sufficient ce (live: RegionSet.t) (svm: sv_map) : Prop :=
-  forall rph ph vs mut,
-    (* Do we need to say that rph must be live? *)
-    get_owner_sval_map rph svm = OK (sv_ref mut ph vs) ->
-    (** TODO: The deref of rph must be not in [vs], otherwise we
-    cannot prove the premise of not In in the following conclusion. *)    
-    forall ph1 vs1,
-      get_owner_path_sv_map ph1 svm = OK (ph, vs1) ->
-      is_live_path live (svm_to_tenv svm) ph1 = true ->
-      mutable_path ce svm ph1 = true ->
-      (* The views of ph1, i.e., vs1 does not contain reborrowed path
-      of rph *)
-      ~ In (append_proj proj_deref rph) vs1 ->
-      In ph1 vs.
+Fixpoint all_splits {A} (l : list A) : list (list A * list A) :=
+  match l with
+  | nil => nil
+  | x :: xs => (x::nil, xs) :: map (fun '(p,s) => (x::p, s)) (all_splits xs)
+  end.
+
+
+Definition dominators_of_owner_projections (l: list projection) : list (list projection * list projection) :=
+  filter (fun '(_, s) => in_dec projection_eq proj_deref s) (all_splits l).
+
+
+Inductive reachable_from_dominators (fpg: fp_graph) : path -> path -> Prop :=
+| reachable_from_dominators_intro: forall id1 pjl1 id2 pjl dom_pjl suf_pjl vs,
+    In (dom_pjl, suf_pjl) (dominators_of_owner_projections pjl) ->
+    get_owner_path_map (id1, pjl1) fpg = OK ((id2, dom_pjl), vs) ->
+    reachable_from_dominators fpg (id1, pjl1 ++ suf_pjl) (id2, pjl).
+    
+
+Record alias_graph_views_inv (fpg: fp_graph) (ph: path) (vs: views) (tgt: path) : Prop :=
+  { alias_graph_views_precise: forall ph1,
+      In ph1 vs ->
+      exists vs1, 
+        get_owner_path_map ph1 fpg = OK (tgt, vs1)
+        /\ mutable_path ph1 fpg = OK true;
+    
+    alias_graph_views_owner: In tgt vs;
+
+    (* all dominators path is included in vs *)
+    alias_graph_views_adequate: forall ph1,
+      reachable_from_dominators fpg ph1 tgt ->
+      mutable_path ph1 fpg = OK true ->
+      In ph1 vs;
+
+    alias_graph_views_stack_discipline: forall ph1 vs1,
+      get_owner_path_map ph1 fpg = OK (tgt, vs1) ->
+      mutable_path ph1 fpg = OK true ->
+      ~ In ph1 vs ->
+      In ph vs1;                (* If [ph] is a temporary path, then
+      it cannot be in [vs1], which means that [ph1] must be in [vs],
+      i.e., all the paths reachable to tgt is included in the views
+      [vs] of [ph] *)
+
+ }.
+
+Definition borrow_check_views_inv (fpg: fp_graph) : Prop :=
+  forall ph tgt vs,
+    get_owner_path_map ph fpg = OK (tgt, vs) ->
+    mutable_path ph fpg = OK true ->
+    alias_graph_views_inv fpg ph vs tgt.
 
 (** Type invariants: the reference type must be equal to the type it
 points to *)
 
-Definition svm_ref_type_inv ce (live: RegionSet.t) (svm: sv_map) : Prop :=
-  forall ph1 ph2 ph3 vs2 vs3 r mut ty1,
-    get_owner_path_sv_map ph1 svm = OK (ph2, vs2) ->
-    get_owner_sval_map ph2 svm = OK (sv_ref mut ph3 vs3) ->
-    is_live_path live (svm_to_tenv svm) ph1 = true ->
-    wt_path ce (svm_to_tenv svm) ph1 = OK (Treference r mut ty1) ->
-    exists ty2, wt_path ce (svm_to_tenv svm) ph2 = OK ty2 /\ type_eq_except_origins ty1 ty2 = true.
 
+(* Definition fpg_ref_type_inv ce (fpg: fp_graph) : Prop := *)
+(*   forall ph1 ph2 vs2 ty1, *)
+(*     get_owner_path_map ph1 fpg = OK (ph2, vs2) -> *)
+(*     wt_path ce (fpg_to_tenv fpg) ph1 = OK ty1 -> *)
+(*     exists ty2, wt_path ce (fpg_to_tenv fpg) ph2 = OK ty2 /\ type_eq_except_origins ty1 ty2 = true. *)
 
-(** Footprint can be seen as a rich form of structured value in
-RustIRspec, which contains extra permission information. We can use
-[fp_to_sval] to remove this information. *)
-
-
-(* Translate footprint to structured value *)
-Fixpoint fp_to_sval (fp: footprint) : sval :=
-  match fp with
-  | fp_emp
-  | fp_uninit _ _ => sv_bot
-  | fp_scalar _ v => sv_scalar v
-  | fp_box _ fp1 => sv_box (fp_to_sval fp1)
-  | fp_struct id fpl => sv_struct id (map (fun '(fid, (_, ffp)) => (fid, fp_to_sval ffp)) fpl)
-  | fp_enum id _ fid _ ffp => sv_enum id fid (fp_to_sval ffp)
-  | fp_ref mut _ _ ph vs => sv_ref mut ph vs 
-  | fp_object id obj exposed => sv_object id (mem_to_pure_repr (ame id) obj) (map (fun '(fid, (_,
-ty, ffp)) => (fid, (ty, fp_to_sval ffp))) exposed)
-  end.
-
-Definition fpm_to_svm (fpm: fp_map) : sv_map :=
-  PTree.map1 (fun '(_, r, ty, fp) => (r, ty, fp_to_sval fp)) fpm.
 
 (* If a reference is live, then its value is the same as the location
-of the owner it points to *)
-Definition fpm_ref_loc_inv (live: RegionSet.t) (fpm: fp_map) : Prop :=
-  forall ph1 ph2 ph3 b0 ofs0 b ofs mut vs2 vs,
-    get_owner_path_sv_map ph1 (fpm_to_svm fpm) = OK (ph2, vs2) ->
-    get_owner_loc_footprint_map ph2 fpm = Some (b0, ofs0, fp_ref mut b ofs ph3 vs) ->
-    is_live_path live fpm ph1 = true ->
-    exists fp, get_owner_loc_footprint_map ph3 fpm = Some (b, ofs, fp)
-          (* Should we write it as an invariant on sval map instead of
-          on the footprint map? *)
-          /\ deep_owned fp = true.
+of the owner it points to. We use fpg to represent the footprint map
+with the temporary variables storing the temporary value evaluated by
+the expression and fpm to compute the address.  *)
+(* Definition fpm_ref_loc_inv (fpg: fp_graph) (fpm: fp_map) : Prop := *)
+(*   forall ph1 ph2 b ofs mut vs, *)
+(*     @get_owner_footprint_map ame ph1 fpg = OK (fp_ref mut b ofs (Some ph2) vs) -> *)
+(*     exists fp, get_owner_loc_footprint_map ph2 fpm = OK (b, ofs, fp). *)
 
 
 (* The invariant established and preserved by the borrow checking *)
-Record borrow_check_inv ce (live: RegionSet.t) (le: LOrgEnv.t) (svm: sv_map) (fpm: fp_map) : Prop :=
-  { borrowck_approximation: sound_loan_analysis ce live le svm;
-    borrowck_sufficient_views: alias_graph_views_sufficient ce live svm;
-    borrowck_svm_ref_type_inv: svm_ref_type_inv ce live svm;
-    borrowck_fpm_ref_loc_inv: fpm_ref_loc_inv live fpm; }.
+Record borrow_check_inv (fpm: fp_map) : Prop :=
+  { borrowck_views_inv: borrow_check_views_inv fpm; }.
+    (* borrowck_fpg_ref_type_inv: fpg_ref_type_inv ce fpm; *)
+    (* borrowck_fpm_ref_loc_inv: fpm_ref_loc_inv fpm fpm; }. *)
 
 End ADT_ENV.
-
-Coercion fp_to_sval : footprint >-> sval.
-Coercion fpm_to_svm : fp_map >-> sv_map.
-
-
-(* Old version of the borrow check invariant which contains properties about stacked borrow
-
-Definition loan_approx (fpm: fp_map) (l: loan) (ph: path) : Prop :=
-  match l, extern_loc_region fpm ph with
-  | Lintern _ p, None =>
-      (* TODO: use path uniformly *)
-      let (id1, pj1) := path_of_place p in
-      let (id2, pj2) := ph in
-      id1 = id2 /\ projections_contain pj1 pj2 = true
-  | Lextern org1, Some org2 =>
-      org1 = org2 
-  | _, _ => False
-  end.
-
-
-(* ph is the location the stack resides in *)
-Inductive borstk_approx_loans ce (live: RegionSet.t) (orgst: LOrgSt.t) (fpm: fp_map) (stk: BorStkPerm.t) (ph: path) (it: BorStkPerm.item) : Prop :=
-| borstk_approx_loans_intro: forall stk1 stk2 ls,
-    orgst = Live ls ->
-    (* The item is in the stack. What about the uniqueness of this item? *)
-    (** We should prove that all suffix of stk containing it :: stk2
-    also satisfies this property *)
-    stk = stk1 ++ it :: stk2 ->
-    (* all valid Unique items in stk2 are approximated by ls *)
-    (forall b ofs ph1 ph2 fp pj,
-        In (BorStkPerm.Unique (b, ofs)) stk2 ->
-        (* ph2 is a node in the footprint tree *)
-        get_owner_loc_footprint_map ph2 fpm = Some (b, ofs, fp) ->
-        (* ph2 is reachable via an arbitary path [ph1] *)
-        get_owner_path_map ph1 fpm = Some ph2 ->
-        (* We should know how ph2 reaches ph; the projections should
-        have the form [proj_deref; proj_field/downcast^*] *)
-        get_owner_path fpm ph2 pj fp = Some ph ->
-        (* ph1 is mutable *)
-        mutable_path ce fpm ph1 = true ->
-        (* ph1 is live *)
-        is_live_path live fpm ph1 = true ->
-        (* The conclusion is that ls contains a loan that is prefix of
-        [ph1; proj_deref]. TODO: what if the location of this stk is
-        within some fields? *)
-        exists ln, 
-          LoanSet.In ln ls 
-          (* If ph1 is from external locations then ln must be
-          Lextern('a) where 'a is the region of this external
-          location; otherwise ln is a prefix of ph1. We use
-          loan_of_path to compute the loan of this path (imagine that
-          it is borrow?) *)
-          /\ loan_approx fpm ln ph2) ->
-    borstk_approx_loans ce live orgst fpm stk ph it.
-  
-Local Open Scope map_scope.
-
-Definition stkbor_ref_inv ce (live: RegionSet.t) (le: LOrgEnv.t) (fpm: fp_map) (stk_mem: bor_stacks) :=
-  forall ph1 ph2 org mut ty, 
-    wt_path ce fpm ph1 = OK (Treference org mut ty) ->
-    (* ph1 is a live path *)
-    is_live_path live fpm ph1 = true ->
-    get_owner_path_map ph1 fpm = Some ph2 ->
-    (* The footprint at ph2 is fp_ref *)
-    forall rb rofs ph3, 
-      get_owner_footprint_map ph2 fpm = Some (fp_ref rb rofs ph3) ->
-      forall del,
-        0 <= del < sizeof ce ty ->
-        exists stk, 
-          stk_mem # rb ## (rofs + del) = Some stk
-          (** Since path ph2 is live, it must appear in the
-              stack at (rb, rofs + del). *)
-          /\ borstk_approx_loans ce live (LOrgEnv.get org le) fpm stk ph3 (BorStkPerm.to_item mut (rb,rofs)).
-
-
-Definition stkbor_box_inv (live: RegionSet.t) (le: LOrgEnv.t) (fpm: fp_map) (stk_mem: bor_stacks) :=
-  forall ph b sz fp,
-    get_owner_footprint_map ph fpm = Some (fp_box b sz fp) ->
-    not_fp_emp fp = true ->
-    forall del,
-      0 <= del < sz ->
-      exists stk, 
-        (* The last element of the borrow stack of a heap block must
-        be the box pointer itself *)
-        stk_mem # b ## del = Some (stk ++ [BorStkPerm.Unique (b,0)]).
-
-(* If a reference is live, then its value is the same as the location
-of the owner it points to *)
-Definition fpm_ref_inv (live: RegionSet.t) (fpm: fp_map) : Prop :=
-  forall ph1 b ofs ph2,
-    get_owner_footprint_map ph1 fpm = Some (fp_ref b ofs ph2) ->
-    is_live_path live fpm ph1 = true ->
-    exists fp, get_owner_loc_footprint_map ph2 fpm = Some (b, ofs, fp). 
-
-(* The invariant established and preserved by the borrow checking *)
-Record borrow_check_inv ce (live: RegionSet.t) (le: LOrgEnv.t) (fpm: fp_map) (stk_mem: bor_stacks) : Prop :=
-  { borrowck_stkbor_ref: stkbor_ref_inv ce live le fpm stk_mem;
-    borrowck_fpm_ref: fpm_ref_inv live fpm }.
-
-*) 
