rustfrontend/BorrowCheckSim.v
@@ -1,4 +1,4 @@
-Require Import Coqlib .
+Require Import Coqlib.
 Require Import Errors Maps.
 Require Import Values.
 Require Import Integers.
@@ -14,7 +14,7 @@ Require Import Errors.
 Require Import InitDomain InitAnalysis.
 Require Import RustIRspec RustIRsem.
 Require Import RustIRspecMem.
-(* Require Import BorrowCheckInv. *)
+Require Import BorrowCheckInv.
 Require Import Wfsimpl.
 Require Import Separation Listmisc.
 (* use free_list related lemmas *)
@@ -578,7 +578,7 @@ Inductive match_cont: (@RustIRspec.cont ame) -> cont -> massert -> Prop :=
 with match_stacks : (@RustIRspec.cont ame) -> cont -> massert -> Prop :=
 | match_stacks_call: forall f k tk MP1 MP2 phl ns fpm fpm1 p
     (* We should set fp_emp to the inout parameters *)
-    (FPM: clear_fpm_passed_ref_footprint fpm (map fst phl) = OK fpm1)
+    (FPM: clear_fpm_passed_ref_footprint fpm (map (fun '(id, (ph, _)) => ph) phl) = OK fpm1)
     (COH: coherent_fpm ge fpm1 MP1)
     (CONT: match_cont k tk MP2),
     match_stacks (RustIRspec.Kcall p f phl ns fpm k) (Kcall (Some p) f fpm tk) (MP1 ** MP2)
@@ -591,39 +591,43 @@ Inductive match_states: state_spec -> state -> Prop :=
     (MCONT: match_cont k tk FMP)
     (MPRED: m |= MP ** FMP),
     match_states (RustIRspec.State f s k ns fpm (Mem.support m)) (State f s tk fpm m)
-| match_callstate: forall vf fd orgs org_rels tyargs tyres cconv m fpl args k MP1 MP2 MP3 inout_fpl inout_locs inout_params tk fun_id tyl
+| match_callstate: forall vf fd orgs org_rels tyargs tyres cconv m fpl args k MP1 MP2 MP3 inout_fpm tk fun_id
     (* TODO: show that fun_id also points to this function *)
     (FUNC: Genv.find_funct ge vf = Some fd)    
     (FUNTY: type_of_fundef fd = Tfunction orgs org_rels tyargs tyres cconv)
     (* arguments are semantics well typed *)
     (WTVAL_LIST: sem_wt_val_list ce fpl args MP1)
     (** output memory locations are sem_wt_loc *)
-    (INOUTLOCS: map (fun '(b, ofs, _, _, _) => (b, ofs)) inout_params = inout_locs)
-    (INOUTFPL: map snd inout_params = inout_fpl)
-    (WTLOC_LIST: sem_wt_loc_list ce inout_locs inout_fpl MP2)
+    (* (INOUTLOCS: map (fun '(b, ofs, _, _, _) => (b, ofs)) inout_params = inout_locs) *)
+    (* (INOUTFPL: map snd inout_params = inout_fpl) *)
+    (* (WTLOC_LIST: sem_wt_loc_list ce inout_locs inout_fpl MP2) *)
+    (INOUT_FPM: coherent_fpm ce inout_fpm MP2)
     (* (ANORM: val_casted_list args tyargs) *)
-    (WTFP: list_forall2 (wt_footprint ce) (type_list_of_typelist tyargs) fpl)
-    (INOUT_TYL: map (fun '(_, _, ty, _) => ty) inout_params = tyl)
-    (WT_INOUTFP: list_forall2 (wt_footprint ce) tyl inout_fpl)
+    (WTFP: list_forall2 (wt_footprint ce inout_fpm) (type_list_of_typelist tyargs) fpl)
+    (* (INOUT_TYL: map (fun '(_, _, ty, _) => ty) inout_params = tyl) *)
+    (** TODO: move this property to borrow check invariant *)
+    (WT_INOUTFPM: wt_fpm ce inout_fpm)
     (MPRED: m |= MP1 ** MP2 ** MP3)
     (STK: match_stacks k tk MP3),
     (* also disjointness of fpl and fpf *)
-    match_states (RustIRspec.Callstate fun_id fpl inout_params (Mem.support m) k) (Callstate vf args tk m)
-| match_returnstate: forall sg m k retty vfp v MP1 MP2 MP3 tk inout_locs inout_params inout_tyl inout_fpl
+    match_states (RustIRspec.Callstate fun_id fpl inout_fpm (Mem.support m) k) (Callstate vf args tk m)
+| match_returnstate: forall sg m k retty vfp v MP1 MP2 MP3 tk inout_fpm
     (* For now, all function must have return type *)
     (RETY: typeof_cont_call (rs_sig_res sg) tk = retty)
     (WTVAL: sem_wt_val ce vfp v MP1)
     (** inout memory locations are sem_wt_loc *)
-    (INOUTLOCS: map (fun '(b, ofs, _, _, _) => (b, ofs)) inout_params = inout_locs)
-    (INOUTFPL: map snd inout_params = inout_fpl)
-    (INOUT_TYL: map (fun '(_, _, ty, _) => ty) inout_params = inout_tyl)
-    (WTLOC_LIST: sem_wt_loc_list ce inout_locs inout_fpl MP2)
+    (* (INOUTLOCS: map (fun '(b, ofs, _, _, _) => (b, ofs)) inout_params = inout_locs) *)
+    (* (INOUTFPL: map snd inout_params = inout_fpl) *)
+    (* (INOUT_TYL: map (fun '(_, _, ty, _) => ty) inout_params = inout_tyl) *)
+    (* (WTLOC_LIST: sem_wt_loc_list ce inout_locs inout_fpl MP2) *)
+    (INOUT_FPM: coherent_fpm ce inout_fpm MP2)
     (* (CAST: val_casted v retty) *)
-    (WTFP: wt_footprint ce retty vfp)
-    (WT_INOUTFP: list_forall2 (wt_footprint ce) inout_tyl inout_fpl)
+    (WTFP: wt_footprint ce inout_fpm retty vfp)
+    (* (WT_INOUTFP: list_forall2 (wt_footprint ce) inout_tyl inout_fpl) *)
+    (WT_INOUTFPM: wt_fpm ce inout_fpm)
     (MPRED: m |= MP1 ** MP2 ** MP3)    
     (STK: match_stacks k tk MP3),
-    match_states (RustIRspec.Returnstate vfp inout_params (Mem.support m) k) (Returnstate v tk m).
+    match_states (RustIRspec.Returnstate vfp inout_fpm (Mem.support m) k) (Returnstate v tk m).
 
 
 (** Properties of evaluating place and expressions  *)
@@ -634,7 +638,7 @@ Ltac destr_get_fpm fpm id :=
   let GFP := fresh "GFP" in
   destruct (fpm ! id) as [((((?b & ?ofs) & ?r) & ?ty) & ?fp)|] eqn: GFP;
   match goal with
-  | [H : context G [fpm_to_svm fpm] |- _ ] =>
+  | [H : context G [fpm_to_fpg] |- _ ] =>
       setoid_rewrite PTree.gmap1 in H;
       rewrite GFP in H;
       simpl in H
@@ -645,43 +649,55 @@ Ltac destr_path_of_place p :=
 
 
 Ltac destr_find_field H :=
-  destruct find_field as [?p|] eqn: FIND in H; try congruence.
+  destruct find_field as [((?lo & ?hi) & ?ffp)|] eqn: FIND in H; try congruence.
 
 (* Graph properties of sv_map *)
 
-Lemma get_owner_loc_footprint_map_to_sval: forall ph fpm b ofs fp sv,
-    get_owner_loc_footprint_map ph fpm = Some (b, ofs, fp) ->
-    get_owner_sval_map ph fpm = OK sv ->
-    fp_to_sval fp = sv.
-Admitted.
 
-Lemma get_owner_path_sv_map_inv: forall id phl (svm: sv_map) ph vs,
-    get_owner_path_sv_map (id, phl) svm = OK (ph, vs) ->
-    exists r ty sv, 
-      svm ! id = Some (r, ty, sv)
-      /\ get_owner_path svm (id, nil) phl sv nil = OK (ph, vs).
+Lemma get_owner_path_map_inv: forall id phl (fpg: fp_graph) ph vs,
+    get_owner_path_map (id, phl) fpg = OK (ph, vs) ->
+    exists (fp: footprint),
+      fpg ! id = Some fp
+      /\ get_owner_path fpg (id, nil) phl fp nil = OK (ph, vs).
 Admitted.
 
 
-Ltac inv_get_owner_path_svm H :=
+Ltac inv_get_owner_path_fpm H :=
   let GPH := fresh "GPH" in
-  eapply get_owner_path_sv_map_inv in H as GPH;
-  destruct GPH as (?r & ?ty & ?sv & ?G1 & ?G2).
+  eapply get_owner_path_map_inv in H as GPH;
+  destruct GPH as (?fp & ?G1 & ?G2).
 
 (* If a path can be reached via (phl1 ++ phl2) then this reachable
 path can be divided into two parts: one is reached from phl1 and one
 is reach from phl2 *)
-Lemma get_owner_path_app_inv: forall phl1 phl2 ph1 ph3 sv1 vs1 vs3 (svm: sv_map),
-    get_owner_path svm ph1 (phl1 ++ phl2) sv1 vs1 = OK (ph3, vs3) ->
+Lemma get_owner_path_app_inv: forall phl1 phl2 ph1 ph3 sv1 vs1 vs3 (fpm: fp_map),
+    get_owner_path fpm ph1 (phl1 ++ phl2) sv1 vs1 = OK (ph3, vs3) ->
     exists ph2 vs2 sv2,
-      get_owner_path svm ph1 phl1 sv1 vs1 = OK (ph2, vs2) 
-      /\ get_owner_sval_map ph2 svm = OK sv2 
-      /\ get_owner_path svm ph2 phl2 sv2 vs2 = OK (ph3, vs3).
+      get_owner_path fpm ph1 phl1 sv1 vs1 = OK (ph2, vs2) 
+      /\ get_owner_footprint_map ph2 fpm = OK sv2 
+      /\ get_owner_path fpm ph2 phl2 sv2 vs2 = OK (ph3, vs3).
 Admitted.
 
-Lemma get_owner_path_for_owner: forall svm ph sv,
-    get_owner_sval_map ph svm = OK sv ->
-    exists vs, @get_owner_path_sv_map ae ph svm = OK (ph, vs).
+Lemma get_owner_path_for_owner: forall (fpm: fp_map) ph fp,
+    get_owner_footprint_map ph fpm = OK fp ->
+    exists vs, get_owner_path_map ph fpm = OK (ph, vs).
+Admitted.
+
+Lemma get_owner_loc_footprint_map_eq: forall (fpm: fp_map) ph b ofs fp,
+    get_owner_loc_footprint_map ph fpm = OK (b, ofs, fp) ->
+    get_owner_footprint_map ph fpm = OK fp.
+Admitted.
+
+Lemma get_owner_loc_footprint_map_app: forall id phl1 phl2 b1 ofs1 fp1 b2 ofs2 fp2 fpm,
+    get_owner_loc_footprint_map (id, phl1) fpm = OK (b1, ofs1, fp1) ->
+    get_owner_loc_footprint phl2 fp1 b1 ofs1 = OK (b2, ofs2, fp2) ->         
+    get_owner_loc_footprint_map (id, phl1 ++ phl2) fpm = OK (b2, ofs2, fp2).
+Admitted.
+
+Lemma get_owner_loc_footprint_map_wt: forall phl id fpm b ofs fp,
+    get_owner_loc_footprint_map (id, phl) fpm = OK (b, ofs, fp) ->
+    exists ty, wt_path ce fpm (id, phl) = OK ty
+          /\ wt_footprint ce fpm ty fp.
 Admitted.
 
 Ltac inv_get_owner_path_app H :=
@@ -690,47 +706,45 @@ Ltac inv_get_owner_path_app H :=
   let GVAL := fresh "GVAL" in
   let GPH2 := fresh "GPH2" in
   eapply get_owner_path_app_inv in H as GPH;
-  destruct GPH as (?ph & ?vs & ?sv & GPH1 & GVAL & GPH2).
+  destruct GPH as (?ph & ?vs & ?fp & GPH1 & GVAL & GPH2).
 
-Lemma get_owner_sval_map_loc : forall phl id (fpm: fp_map) sv
-    (GET_PH: get_owner_sval_map (id, phl) fpm = OK sv),
-    exists b ofs fp, 
-      get_owner_loc_footprint_map (id, phl) fpm = Some (b, ofs, fp).
-Admitted.
+(* Lemma get_owner_sval_map_loc : forall phl id (fpm: fp_map) fp *)
+(*     (GET_PH: get_owner_footprint_map (id, phl) fpm = OK fp), *)
+(*     exists b ofs fp,  *)
+(*       get_owner_loc_footprint_map (id, phl) fpm = Some (b, ofs, fp). *)
+(* Admitted. *)
 
-Lemma get_owner_path_sv_map_eval_place: forall (p: place) fpm vs ph m live MP f externs
+Lemma get_owner_path_map_eval_place: forall (p: place) fpm vs ph m MP
     (COH: coherent_fpm ce fpm MP)
     (MPRED: m |= MP)
-    (FPM_INV: fpm_ref_loc_inv live fpm)
+    (WT_FPM: wt_fpm ce fpm)
     (WTP: wt_place fpm ce p)
-    (WF_FPM: wf_fpm f externs fpm)
-    (** TODO: show that regions in p are live *)
-    (LIVE_PH: is_live_path live fpm p = true)
-    (GET_PH: get_owner_path_sv_map p fpm = OK (ph, vs)),
+    (GET_PH: get_owner_path_map p fpm = OK (ph, vs)),
     exists b ofs fp, 
-      get_owner_loc_footprint_map ph fpm = Some (b, ofs, fp)
+      get_owner_loc_footprint_map ph fpm = OK (b, ofs, fp)
       /\ eval_place ce fpm m p b (Ptrofs.repr ofs).
 Proof.  
   induction p; intros.
-  - simpl in *. destr_get_fpm fpm i; try congruence. inv GET_PH.
+  - simpl in *. 
+    destr_get_fpm fpm i; try congruence. inv GET_PH.
     simpl. rewrite GFP. exists b, ofs, fp. split; auto.
     inv WTP.
     (** TODO: prove that i is a local variable *)
     admit.
   - simpl in GET_PH.
     destr_path_of_place p.
-    inv_get_owner_path_svm GET_PH.
+    inv_get_owner_path_fpm GET_PH.
     inv_get_owner_path_app G2.
-    inv WTP.
-    simpl in LIVE_PH. rewrite POP in LIVE_PH. 
+    inv WTP.    
     exploit IHp. 1-6: eauto.
     simpl. rewrite G1. eauto.
     intros (b1 & ofs1 & fp1 & A1 & A2).
-    (* structure of sv0: how to prove that sv0 must not be opaque object? *)
-    simpl in GPH2. destruct sv0; try congruence.
-    destr_find_field GPH2. inv GPH2.
-    exploit get_owner_loc_footprint_map_to_sval; eauto. intros SVEQ.
-    destruct fp1; simpl in SVEQ; inv SVEQ.
+    (* structure of fp0: how to prove that fp0 must not be opaque
+    object? *)
+    simpl in GPH2. destruct fp0; try congruence.
+    destr_find_field GPH2. inv GPH2.    
+    exploit get_owner_loc_footprint_map_eq. eauto. intros A3.
+    rewrite A3 in GVAL. inv GVAL.
     (* remaining proof: get_owner_loc_footprint_map_app and getting
     the field offset *)
     admit.
@@ -739,57 +753,56 @@ Proof.
   (* Pdefer *)
   - simpl in GET_PH.
     destr_path_of_place p.
-    inv_get_owner_path_svm GET_PH.
+    inv_get_owner_path_fpm GET_PH.
     inv_get_owner_path_app G2.
     inv WTP.
-    simpl in LIVE_PH. rewrite POP in LIVE_PH.     
     exploit IHp; eauto.
     simpl. rewrite G1. eauto.
     intros (b1 & ofs1 & fp1 & A1 & A2).
-    (* structure of sv0 *)
-    simpl in GPH2. destruct sv0; try congruence. inv GPH2.
-    (* sv_box *)
-    + exploit get_owner_loc_footprint_map_to_sval; eauto. intros SVEQ.
-      destruct fp1; simpl in SVEQ; inv SVEQ.
+    (* structure of fp0 *)
+    simpl in GPH2. destruct fp0; try congruence.
+    (* fp_box *)
+    + inv GPH2.
+      exploit get_owner_loc_footprint_map_eq; eauto. intros A3.
+      rewrite A3 in GVAL. inv GVAL.
+      (** TODO: we need some theorem like
+      get_owner_loc_footprint_map_sem_wt_split *)
       destruct ph0 as (?id & ?ph).
       exploit (@get_owner_loc_footprint_map_sem_wt_split ame); eauto.
       intros (mp1 & mp2 & B1 & B2).
       inv B1.
       rewrite B2, EQV in MPRED.
       exploit load_rule. eapply MPRED. intros (?v & C1 & C2). subst.
-      exists b, 0, fp1. split.
-      (** we should prove that fp1 is not emp. This properties should
-      be implied by dominators_owned *)
-      admit.
-      econstructor; eauto. 
-      (** TODO: prove by wt_footprint? *)
-      assert (PTY: typeof_place p = Tbox t) by admit.
-      rewrite PTY. econstructor. reflexivity.
-      simpl. rewrite Ptrofs.unsigned_repr. eauto. 
-      (* prove by hasvalue *)
-      admit.
-    (* sv_ref *)
-    + exploit get_owner_loc_footprint_map_to_sval; eauto. intros SVEQ.
-      destruct fp1; simpl in SVEQ; inv SVEQ.
+      exists b, 0, fp0. split.
+      * eapply get_owner_loc_footprint_map_app; eauto.
+      * econstructor; eauto.
+        (** TODO: prove by wt_footprint? *)
+        assert (PTY: typeof_place p = Tbox t) by admit.
+        rewrite PTY. econstructor. reflexivity.
+        simpl. rewrite Ptrofs.unsigned_repr. eauto.
+        (* prove by hasvalue *)
+        admit.
+    (* fp_ref *)
+    + destruct ph1 as [?ph1|]; try congruence.
       monadInv GPH2.
+      exploit get_owner_loc_footprint_map_eq; eauto. intros A3.
+      rewrite A3 in GVAL. inv GVAL.
       destruct ph0 as (?id & ?ph).
       exploit (@get_owner_loc_footprint_map_sem_wt_split ame); eauto.
       intros (mp1 & mp2 & B1 & B2).
       destruct ph as (?id & ?ph).
-      (* Use invariant for reference *)
-      exploit (FPM_INV (pid, phl)). simpl. rewrite G1. eauto. eauto.
-      (* live path *)
-      eauto.
-      intros (?fp & GREF & DEEP_OWN).
-      exists b, ofs, fp. split; auto.
       inv B1.
       rewrite B2, EQV in MPRED.
       exploit load_rule. eapply MPRED. intros (?v & C1 & C2). subst.
+      (* Use invariant for reference *)
+      exploit get_owner_loc_footprint_map_wt; eauto.
+      intros (ty & WT3 & WT4). inv WT4.
+      exists b, ofs, fp0. split; auto.
       econstructor; eauto. 
-      (** TODO: prove by wt_footprint? *)
-      assert (PTY: exists org, typeof_place p = Treference org mut t) by admit.
-      destruct PTY as (org & PTY).
-      rewrite PTY. econstructor. reflexivity.
+      (** TODO: may be difficult *)
+      assert (PTY1: exists org, typeof_place p = Treference org mut t) by admit.
+      destruct PTY1 as (org1 & PTY2).
+      rewrite PTY2. econstructor. reflexivity.
       simpl. rewrite Ptrofs.unsigned_repr. eauto. 
       admit.
   (* Pdowncast *)
